\documentclass[aps,twocolumn]{revtex4}
\usepackage{graphicx}
\usepackage{amssymb,amsfonts,amsmath,amsthm}
\usepackage{chemarr}
\usepackage{bm}
\usepackage{pslatex}
\usepackage{mathptmx}
\usepackage{xfrac}

%% concentration notations
\newcommand{\mymat}[1]{\boldsymbol{#1}}
\newcommand{\mytrn}[1]{{#1}^{\mathsf{T}}}
\newcommand{\myvec}[1]{\overrightarrow{#1}}
\newcommand{\mygrad}{\vec{\nabla}}
\newcommand{\myhess}{\mathcal{H}}


\begin{document}
\title{Thoughts for Power Spectrum Estimation}
\maketitle


\section{Rectifying a signal}
Let us assume that we have $M$ points of data $f_1,\ldots,f_M$, iso-sampling $f(t)$ over the interval $[0;T]$.
We also assume that the periodic part of $f$ is supported by a polynomial part.
We build the function
\begin{equation}
	g(t) = f(t) - \sum_{k=1}^K a_k t^{(k-1)}
\end{equation}
and the coefficients are determined by the minimization of
\begin{equation}
\int_0^T g(t)^2\,dt.
\end{equation}
We must set
\begin{equation}
	\forall j,\; 0 = \int_0^T g(t)\dfrac{\partial g}{\partial a_j} dt
\end{equation}
or
\begin{equation}
	\int_0^T t^{(j-1)} f(t) dt = \sum_{k=1}^K a_k \int_{0}^T t^{(j+k-2)} \; dt 
\end{equation}
which reads
\begin{equation}
	\sum_{i=1}^M 
	\left\lbrack 
	\dfrac{i^j - (i-1)^{j}}{j}	\right\rbrack
 f_i = \sum_{k=1}^K \dfrac{M^{j+k-1}}{j+k-1} a_k
\end{equation}

We have
\begin{equation}
\mymat{\mu} \vec{a} = \mymat{\sigma}\vec{f}
\end{equation}
with
\begin{equation}
	\mymat{\mu}_{j,k} = \dfrac{M^{j+k-1}}{j+k-1}
\end{equation}
and
\begin{equation}
	\mymat{\sigma}_{j,i} = \dfrac{i^j - (i-1)^{j}}{j}
\end{equation}

\section{Local Maximum Refinement}
Let us assume that $i$ is the index of a local maximum $y_i$ at coordinate $x_i$.
We define
\begin{equation}
	\alpha = \dfrac{x_{i}-x{i-1}}{x_{i+1}-x_{i-1}},
\end{equation}
\begin{equation}
	\beta  = y_i - y_{i-1}
\end{equation}
and
\begin{equation}
	\gamma = y_{i+1} - y_{i-1}.
\end{equation}
We have the reduced parabola
\begin{equation}
	f(X) = \lambda X + \mu X^2
\end{equation}
satisfying
\begin{equation}
	\left\lbrace
	\begin{array}{rcl}
	\beta  & = & \lambda \alpha + \mu \alpha^2\\
	\gamma & = & \lambda+\mu\\
	\end{array}
	\right.
\end{equation}
with a maximum at
\begin{equation}
	X_m = -\dfrac{\lambda}{2\mu}.
\end{equation}
We obtain
\begin{equation}
	\left\lbrace
	\begin{array}{rcl}
	\lambda \alpha(1-\alpha) & = & \beta - \alpha^2\gamma \\
	\mu     \alpha(1-\alpha) & = & -(\beta - \alpha^2\gamma)  \\
	\end{array}
	\right.
\end{equation}
With $\beta>0$, $\gamma\leq\beta$ and $0<\alpha<1$, 
\begin{equation}
	X_m = \dfrac{1}{2} \dfrac{\beta - \alpha^2\gamma}{\beta - \alpha\gamma}
\end{equation}
and
\begin{equation}
	x_m = x_{i-1} + X_m \left(x_{i+1}-x_{i-1}\right).
\end{equation}
We also obtain
\begin{equation}
	y_m = y_{i-1} + \dfrac{1}{4\alpha\left(1-\alpha\right)} \dfrac{\left(\beta - \alpha^2\gamma\right)^2}{\beta-\alpha\gamma}.
\end{equation}


\end{document}