\documentclass[aps]{revtex4}
\usepackage{graphicx}
\usepackage{amssymb,amsfonts,amsmath,amsthm}
\usepackage{chemarr}
\usepackage{bm}
\usepackage{pslatex}
\usepackage{mathptmx}
\usepackage{xfrac}

%% concentration notations
\newcommand{\mymat}[1]{\boldsymbol{#1}}
%\newcommand{\mytrn}[1]{{#1}^{\mathsf{T}}}
\newcommand{\mytrn}[1]{~^{\mathsf{t}}\!{#1}}
\newcommand{\myvec}[1]{\overrightarrow{#1}}
\newcommand{\mygrad}{\vec{\nabla}}
\newcommand{\myhess}{\mathcal{H}}


\begin{document}
\title{Shapes Fitting}

\section{Settings}

We have a set of $N$ points $\vec{A}_i = (x_i,y_i)$ in the plane.

\section{Fitting to a Circle}
This is the method of Kasa and Coope.\\
The algebraic equation of the circle is
\begin{equation}
	x^2+y^2 = ax+by+c
\end{equation}
with $z = x^2+y^2$, we have the multilinear regression problem
\begin{equation}
	z = ax+by+c
\end{equation}
which provides
\begin{equation}
	\label{eq:circ}
	\begin{bmatrix}
	\sum x_i^2 & \sum x_iy_i & \sum x_i\\
	\sum x_iy_i & \sum y_i^2 & \sum y_i\\
	\sum x_i    & \sum y_i & N \\
	\end{bmatrix}
	\begin{bmatrix}
	a\\
	b\\
	c\\
	\end{bmatrix}
	=
	\begin{bmatrix}
	\sum z_i x_i\\
	\sum z_i y_i\\
	\sum z_i\\
	\end{bmatrix}
\end{equation}
Solving \eqref{eq:circ} yields
\begin{equation}
	\left\lbrace
	\begin{array}{rcl}
	x_c & = & \sfrac{a}{2}\\
	y_c & = & \sfrac{b}{2}\\
	r^2 & = & {c}+x_c^2+y_c^2\\
	\end{array}
	\right.
\end{equation}

When adding a weight $w_i$ to each point we have to solve
\begin{equation}
	\label{eq:circ}
	\begin{bmatrix}
	\sum w_i^2 x_i^2 & \sum w_i^2 x_iy_i & \sum w_i^2 x_i\\
	\sum w_i^2 x_iy_i & \sum w_i^2 y_i^2 & \sum w_i^2 y_i\\
	\sum w_i^2x_i    & \sum w_i^2y_i & \sum w_i^2 \\
	\end{bmatrix}
	\begin{bmatrix}
	a\\
	b\\
	c\\
	\end{bmatrix}
	=
	\begin{bmatrix}
	\sum w_i^2z_i x_i\\
	\sum w_i^2z_i y_i\\
	\sum w_i^2z_i\\
	\end{bmatrix}
\end{equation}

\section{Fitting to a Conic}
\subsection{Algebraic definition}
	
\begin{equation}
\label{eq:ell_alg}
	a\,x^2+b\,xy+c\,y^2 + d\,x+e\,y+f = 0
\end{equation}
which requires some constraints on $a,b,c$ to be univocal.
We define rewrite the problem with
\begin{equation}
	\vec{A} = \begin{bmatrix}
	a\\
	b\\
	c\\
	d\\
	e\\
	f
	\end{bmatrix}, 
	\; 
	\vec{Z}_i = 
	\begin{bmatrix}
	x_i^2\\
	x_iy_i\\
	y_i^2\\
	x_i\\
	y_i\\
	1\\
	\end{bmatrix}
\end{equation}
and we want to minimize
\begin{equation}
F^2\left(\vec{A}\right) = \sum_i \left(\vec{A}.\vec{Z}_i\right) 
= \vec{A}^t \underbrace{\left(\sum_i \vec{Z}_i \otimes \vec{Z}_i \right)}_{\bm{S}} \vec{A}
\end{equation}
under the constraint
\begin{equation}
	\vec{A}^t \bm{C} \vec{A} = 1.
\end{equation}
Using the Lagrange multiplier $\lambda$, we need to minimize
\begin{equation}
	\mathcal{L}\left(\vec{A},\lambda\right) = F^2\left(\vec{A}\right) - \lambda \left( \vec{A}^t \bm{C} \vec{A} -1 \right).
\end{equation}
The vectorial part verifies
\begin{equation}
	\bm{S} \vec{A} = \lambda \vec{C} \vec{A}.
\end{equation}
Then $\bm{S}$ must be invertible and we get the eigen problem
\begin{equation}
	\underbrace{\bm{S}^{-1}\bm{C}}_{\displaystyle \bm{M}} \vec{A} = \dfrac{1}{\lambda} \vec{A}.
\end{equation}
To match the constraint and minimize $F^2$, $\bm{M}$ must have a greatest positive eigenvalue
and its associated eigenvector $\vec{U}$, which must also verify 
\begin{equation}
	\vec{U}^t \bm{C} \vec{U} > 0,
\end{equation}
which should be exact...\\
Then we get
\begin{equation}
	\vec{A} = \pm\dfrac{1}{\sqrt{\vec{U}^t \bm{C} \vec{U}}} \vec{U}
\end{equation}

\subsection{Elliptic Reduction}
We can rewrite the quadratic form with
\begin{equation}
	\vec{P} = \begin{bmatrix}
		x\\
		y
		\end{bmatrix},
		\;
		\bm{Q} = \begin{bmatrix}
		a & \dfrac{b}{2}\\
		\dfrac{b}{2} & c
		\end{bmatrix},\;
		\vec{L} = \begin{bmatrix}
		d\\
		e
		\end{bmatrix}
\end{equation}
as
\begin{equation}
	\vec{P}^t \bm{Q} \vec{P} + \vec{L}\cdot\vec{P} + f = 0.
\end{equation}
At the center $\vec{J}$ of the ellipse, the gradient of the quadratic form 
vanishes, so that formally
\begin{equation}
	\bm{Q}\vec{J} = -\dfrac{1}{2}\vec{L}\text{ or }\vec{J} = -\dfrac{1}{2} \bm{Q}^{-1} \vec{L}.
\end{equation}
We now translate the quadratic form with
\begin{equation}
	\vec{P} = \vec{P}' + \vec{J}.
\end{equation}
We get
\begin{equation}
	\left(\vec{P}' + \vec{J}\right)^t \bm{Q} \left(\vec{P}' + \vec{J}\right) +
	\vec{L}\cdot\left(\vec{P}' + \vec{J}\right) + f = 0
\end{equation}
then
\begin{equation}
	\vec{P}'^t \bm{Q} \vec{P'} + 2 \vec{P}'^t \bm{Q} \vec{J} + \vec{J}^t \bm{Q} \vec{J} + 
	\vec{L}\cdot\vec{P}' + \vec{L}\cdot\vec{J} + f = 0.
\end{equation}
Moreover
\begin{equation}
	\vec{P}'^t \bm{Q} \vec{P'} - \vec{L}\cdot\vec{P}' - \dfrac{1}{2} \vec{L}\cdot\vec{J} +
    \vec{L}\cdot\vec{P}' + \vec{L}\cdot\vec{J} + f = 0
\end{equation}
or
\begin{equation}
	\vec{P}'^t \bm{Q} \vec{P} + \dfrac{1}{2} \vec{L}\cdot\vec{J} + f = 0
\end{equation}
and finally
\begin{equation}
	\vec{P}'^t \bm{Q} \vec{P} = \dfrac{1}{4} \vec{L}' \bm{Q}^{-1} \vec{L} -f.
\end{equation}

\end{document}

\section{Fitting to an Ellipse}
\subsection{Algebraic definition}
An algebraic equation is
\begin{equation}
\label{eq:ell_alg}
	a\,x^2+b\,xy+c\,y^2 + d\,x+e\,y+f = 0
\end{equation}
which requires some constraints on $a,b,c$ to be unique.
Let us define 
\begin{equation}
	\vec{A} = 
	\begin{pmatrix}
	a\\
	b\\
	c\\
	\end{pmatrix},\;
	\vec{B} = 
	\begin{pmatrix}
	d\\
	e\\
	f\\
	\end{pmatrix},\;
	\vec{Q} =
	\begin{pmatrix}
	x^2\\
	xy\\
	y^2\\
	\end{pmatrix},\;
	\vec{Z} =
	\begin{pmatrix}
	x\\
	y\\
	1\\
	\end{pmatrix}.
\end{equation}
The equation \eqref{eq:ell_alg} becomes
\begin{equation}
	\vec{A}.\vec{Q} + \vec{B}.\vec{Z} = 0
\end{equation}
We want to minimize
\begin{align}
	F^2\left(\vec{A},\vec{B}\right) & = \sum_{i=1}^N \left(\vec{A}.\vec{Q}_i + \vec{B}.\vec{Z}_i\right)^2\\
	& =  \sum_{i=1}^N \left\lbrack
	\left(\vec{A}.\vec{Q}_i\right)^2 + 2 \left(\vec{A}.\vec{Q}_i\right)\left(\vec{B}.\vec{Z}_i\right) + \left(\vec{B}.\vec{Z}_i\right)^2
	\right\rbrack\\
	& = \vec{A}.\left(\sum_i \vec{Q}_i\otimes\vec{Q}_i\right).\vec{A} +
	 2 \vec{A}.\left(\sum_i \vec{Q}_i\otimes\vec{Z}_i\right).\vec{B} + \vec{B}.\left(\sum_i \vec{Z}_i\otimes\vec{Z}_i\right)\vec{B}.\\
\end{align}
We define the $3\times3$ matrices
\begin{equation}
	\mymat{S}_{qq} =  \vec{Q}_i\otimes\vec{Q}_i,\;\;\mymat{S}_{qz}=\vec{Q}_i\otimes\vec{Z}_i,\;\;\mymat{S}_{zz}=\vec{Z}_i\otimes\vec{Z}_i.
\end{equation}
so that
\begin{align}
	F^2\left(\vec{A},\vec{B}\right)  & = \vec{A}\mymat{S}_{qq}\vec{A} + 2\vec{A}\mymat{S}_{qz}\vec{B} + \vec{B}\mymat{S}_{zz}\vec{B}\\
	 & = \vec{A}\mymat{S}_{qq}\vec{A} + 2\vec{B}\mytrn{\mymat{S}_{qz}}\vec{A} + \vec{B}\mymat{S}_{zz}\vec{B}
\end{align}

Let us minimize $F^2$ under the quadratic constraint
\begin{equation}
	\label{eq:C}
	\vec{A}\mymat{C}\vec{A} = 1
\end{equation}
by setting
\begin{equation}
	L\left(\vec{A},\vec{B}\right) = F^2\left(\vec{A},\vec{B}\right) - \lambda \left( \vec{A}.\mymat{C}.\vec{A} - 1\right).
\end{equation}
We obtain the set of equations
\begin{equation}
	\left\lbrace
	\begin{array}{rcl}
	\mymat{S}_{qq}\vec{A} + \mymat{S}_{qz}\vec{B} & = & \lambda \mymat{C} \vec{A} \\
	\mytrn{\mymat{S}}_{qz}\vec{A} + \mymat{S}_{zz}\vec{B} & = & \vec{0}\\
	\end{array}
	\right.
\end{equation}
The solution are
\begin{equation}
	\vec{B} = -\mymat{S}_{zz}^{-1} \mytrn{\mymat{S}}_{qz}\vec{A} = -\mymat{\beta}\vec{A}
\end{equation}
and
\begin{equation}
	\left(\mymat{S}_{qq} - \mymat{S}_{qz}\mymat{\beta}\right) \vec{A} = \lambda \mymat{C}\vec{A}.
\end{equation}
If we assume that $\mymat{C}$ is invertible then we define
\begin{equation}
	\mymat{M} = \mymat{C}^{-1} \left(\mymat{S}_{qq} - \mymat{S}_{qz}\beta\right)
\end{equation}

Consequently
\begin{equation}
	\lambda \in \mathsf{Spec}\left( M \right)
\end{equation}
and the acceptable eigenvectors $\vec{U}$ must verify
\begin{equation}
	\vec{U}\mymat{C}\vec{U}>0.
\end{equation}
If $\vec{U}$ is an acceptable eigenvector, then a solution $\vec{A}$ is 
\begin{equation}
	\vec{A} = \dfrac{1}{\sqrt{\vec{U}\mymat{C}\vec{U}}} \vec{U}
\end{equation}

If $\vec{A}$ is a solution then
\begin{equation}
	\vec{F}^2 = \vec{A} \left(\mymat{S}_{qq} - \mymat{S}_{qz}\mymat{S}_{zz}^{-1} \mytrn{\mymat{S}}_{qz}\right) \vec{A} = \lambda
\end{equation}
so that $\vec{A}$ is computed from the acceptable eigenvector with the smallest eigenvalue

\subsection{Ellipe reduced equation: TO BE REWRITTEN!!!!}
The quadratic  form is
\begin{equation}
\begin{bmatrix}
x & y\\
\end{bmatrix}
\begin{bmatrix}
 a & \dfrac{b}{2} \\
 \dfrac{b}{2} & c\\
\end{bmatrix}
	\begin{bmatrix}
	x\\
	y\\
	\end{bmatrix}
	+
	\begin{bmatrix}
	x & y\\
	\end{bmatrix}
	\begin{bmatrix}
	d\\
	e\\
	\end{bmatrix}
	+f = 0
\end{equation}
At the center of the ellipse, the gradient of the quadratic form vanishes to that
\begin{equation}
	\begin{bmatrix}
 a & \dfrac{b}{2} \\
 \dfrac{b}{2} & c\\
\end{bmatrix}
\begin{bmatrix}
	x_c\\
	y_c\\
\end{bmatrix}
= -\dfrac{1}{2} 
\begin{bmatrix}
	d\\
	e\\
	\end{bmatrix}.
\end{equation}
Using $x=x'+x_c$ and $y=y'+y_c$
one finds
\begin{equation}
	\begin{bmatrix}
x' & y'\\
\end{bmatrix}
\begin{bmatrix}
 a & \dfrac{b}{2} \\
 \dfrac{b}{2} & c\\
\end{bmatrix}
	\begin{bmatrix}
	x'\\
	y'\\
	\end{bmatrix} 
	+
		\begin{bmatrix}
x_c & y_c\\
\end{bmatrix}
\begin{bmatrix}
 a & \dfrac{b}{2} \\
 \dfrac{b}{2} & c\\
\end{bmatrix}
	\begin{bmatrix}
	x_c\\
	y_c\\
	\end{bmatrix} 
+
	\begin{bmatrix}
x_c & y_c\\
\end{bmatrix}	
\begin{bmatrix}
	d\\
	e\\
	\end{bmatrix}
+
	 f = 0
\end{equation}
and
\begin{equation}
\begin{bmatrix}
x' & y'\\
\end{bmatrix}
\begin{bmatrix}
 a & \dfrac{b}{2} \\
 \dfrac{b}{2} & c\\
\end{bmatrix}
	\begin{bmatrix}
	x'\\
	y'\\
	\end{bmatrix} = \dfrac{1}{4} 
	\begin{bmatrix}
	d & e\\
	\end{bmatrix}
	\begin{bmatrix}
		a & \dfrac{b}{2} \\
 		\dfrac{b}{2} & c\\	\end{bmatrix}^{-1}
	 \begin{bmatrix}
	d\\
	e\\
	\end{bmatrix}- f.
\end{equation}
Since we have an ellipse, there exists $\lambda_X>0$, $\lambda_Y>0$ and an orthogonal matrix $\mymat{Q}$ such that
\begin{equation}
\begin{bmatrix}
 a & \dfrac{b}{2} \\
 \dfrac{b}{2} & c\\
\end{bmatrix}
= \mymat{Q}
\begin{bmatrix}
	\lambda_X & 0 \\
	0  & \lambda_Y \\
\end{bmatrix}
\mytrn{\mymat{Q}}.
\end{equation}
With 
\begin{equation}
	\begin{bmatrix}
	x'\\
	y'\\
	\end{bmatrix}
	=
	\mytrn{\mymat{Q}}
	\begin{bmatrix}
	X\\
	Y\\
	\end{bmatrix}
\end{equation}
and
\begin{equation}
	\begin{bmatrix}
	D \\
	E \\
	\end{bmatrix}
	=
	\mytrn{\mymat{Q}}
	\begin{bmatrix}
	d\\
	e\\
	\end{bmatrix}
\end{equation}
we obtain
\begin{equation}
	\begin{bmatrix}
	x_c\\
	y_c\\
	\end{bmatrix}
	= -\dfrac{1}{2}\mymat{Q}
	\begin{bmatrix}
	D / \lambda_X\\
	E / \lambda_Y\\
	\end{bmatrix}
\end{equation}
and
\begin{equation}
	\lambda_X X^2 + \lambda_Y Y^2 = \dfrac{1}{4}\left(\dfrac{D^2}{\lambda_X} + \dfrac{E^2}{\lambda_Y}\right) - f
\end{equation}

\
\end{document}
